interface_abstraction/Network.thy
@@ -77,403 +77,91 @@ section{*A network consisting of entities*}
         done
     end
 
-   subsection{*Selecting hosts and NetworkBoxes*}
-    text{*select all hosts in an interface set*}
-    definition hosts :: "'v interface set \<Rightarrow> 'v interface set" where
-      "hosts ifaces \<equiv> {e \<in> ifaces. \<exists> x. entity e = Host x}"
-    (*hosts only contains hosts*)
-    lemma "entity ` hosts ifaces = Host ` entity_name ` entity ` hosts ifaces"
-      apply(simp add: hosts_def image_def)
-      apply(rule Set.Collect_cong)
-      apply(simp add: entity_name_def)
-      by fastforce
 
-    definition networkboxes :: "'v interface set \<Rightarrow> 'v interface set" where
-      "networkboxes ifaces \<equiv> {e \<in> ifaces. \<exists> x. entity e = NetworkBox x}"
-    lemma networkboxes_subset: "networkboxes x \<subseteq> x"
-      by(auto simp add: networkboxes_def)
+subsection{*Moving packets*}
+  text{*The following simple model is used. A packet is moved from input interface to input interface.
+        Therefore, two steps are necessary. 
+        1) the entity forwarding function outputs the packet at output interfaces. 
+        2) the packet traverses the link and thus arrives at the next input interface. *}
 
-    subsection{*Moving packets*}
-      text{*The following simple model is used. A packet is moved from input interface to input interface.
-            Therefore, two steps are necessary. 
-            1) the entity forwarding function outputs the packet at output interfaces. 
-            2) the packet traverses the link and thus arrives at the next input interface. *}
+  text{*succ moves packet along links. It is step 2*}
+  definition succ :: "'v network \<Rightarrow> 'v interface \<Rightarrow> ('v interface) set" where
+    "succ N out_iface \<equiv> {in_iface. (out_iface, in_iface) \<in> links N}"
 
-      text{*succ moves packet along links. It is step 2*}
-      definition succ :: "'v network \<Rightarrow> 'v interface \<Rightarrow> ('v interface) set" where
-        "succ N out_iface \<equiv> {in_iface. (out_iface, in_iface) \<in> links N}"
+  lemma succ_subseteq_interfaces: assumes wf_N: "wellformed_network N" shows "succ N x \<subseteq> interfaces N"
+    apply(simp add: succ_def)
+    using wellformed_network.snd_links[OF wf_N] by force
+  lemma succ_subset_networkboxes: "succ N start \<subseteq> networkboxes (succ N start) \<Longrightarrow> succ N start = networkboxes (succ N start)"
+    by(simp add: networkboxes_def, blast)
+  lemma start_notininterfaces_succ_empty: assumes wf_N: "wellformed_network N" shows "start \<notin> interfaces N \<Longrightarrow> succ N start = {}"
+    apply(simp add: succ_def)
+    using wellformed_network.fst_links[OF wf_N] by fastforce
 
-      lemma succ_subseteq_interfaces: assumes wf_N: "wellformed_network N" shows "succ N x \<subseteq> interfaces N"
-        apply(simp add: succ_def)
-        using wellformed_network.snd_links[OF wf_N] by force
-      lemma succ_subset_networkboxes: "succ N start \<subseteq> networkboxes (succ N start) \<Longrightarrow> succ N start = networkboxes (succ N start)"
-        by(simp add: networkboxes_def, blast)
-      lemma start_notininterfaces_succ_empty: assumes wf_N: "wellformed_network N" shows "start \<notin> interfaces N \<Longrightarrow> succ N start = {}"
-        apply(simp add: succ_def)
-        using wellformed_network.fst_links[OF wf_N] by fastforce
+  text{*A packet traverses a hop. It performs steps 1 and 2.*}
+  (*recall: (forward N hdr hop) return the ports where the packet leaves the entity*)
+  definition traverse :: "'v network \<Rightarrow> 'v hdr \<Rightarrow> 'v interface \<Rightarrow> ('v interface) set" where
+    "traverse N hdr hop \<equiv> \<Union> p \<in> (forward N hdr hop). succ N \<lparr>entity = entity hop, port = p\<rparr>"
 
-      text{*A packet traverses a hop. It performs steps 1 and 2.*}
-      (*recall: (forward N hdr hop) return the ports where the packet leaves the entity*)
-      definition traverse :: "'v network \<Rightarrow> 'v hdr \<Rightarrow> 'v interface \<Rightarrow> ('v interface) set" where
-        "traverse N hdr hop \<equiv> \<Union> p \<in> (forward N hdr hop). succ N \<lparr>entity = entity hop, port = p\<rparr>"
-
-      (*traverse jumps over routers, it is not in the links. the forwarding function moves packets in routeres, there is no corresponding link IN an entity for it. *)
-      lemma traverse_subseteq_interfaces: "wellformed_network N \<Longrightarrow> traverse N hdr hop \<subseteq> interfaces N"
-        apply(simp add: traverse_def succ_def)
-        apply(drule wellformed_network.snd_links)
-        by force
-      corollary traverse_finite: assumes wf_N: "wellformed_network N"
-        shows "finite (traverse N hdr hop)"
-        using traverse_subseteq_interfaces[OF wf_N] wellformed_network.finite_interfaces[OF wf_N] by (metis rev_finite_subset)
-
- 
-
-    subsection {*Reachable interfaces*}
-      text{* Traverese performs one step to move a packet. The reachable set defines all reachable entities for a given start node of a packet. *}
-      (* we can allow spoofing by allowing an arbitrary packet header.*)
-      text{*reachable(1): a packet starts at a start node. All directly reachable nodes are reachable.
-            reachable(2): if a hop is reachables, then the next hop is also reachable. *}
-      inductive_set reachable :: "'v network \<Rightarrow> 'v hdr \<Rightarrow> 'v interface \<Rightarrow> ('v interface) set"
-      for N::"'v network" and "pkt_hdr"::"'v hdr" and "start"::"'v interface"
-      where
-        "first_hop \<in> succ N start \<Longrightarrow> first_hop \<in> reachable N pkt_hdr start" |
-        "hop \<in> reachable N pkt_hdr start \<Longrightarrow> next_hop \<in> (traverse N pkt_hdr hop) \<Longrightarrow> next_hop \<in> reachable N pkt_hdr start"
-
-      (*tuned induction rule*)
-      lemmas reachable_induct = reachable.induct[case_names Start Step]
-      thm reachable_induct
-
-      lemma reachable_subseteq_interfaces:
-        assumes wf_N: "wellformed_network N"
-        shows "reachable N pkt_hdr start \<subseteq> interfaces N"
-        proof
-          fix x
-          show "x \<in> reachable N pkt_hdr start \<Longrightarrow> x \<in> interfaces N"
-            apply(induction x rule: reachable_induct)
-            using succ_subseteq_interfaces[OF wf_N] apply blast
-            using traverse_subseteq_interfaces[OF wf_N] by fast
-        qed
-
-    lemma start_notininterfaces_reachableempty: assumes wf_N: "wellformed_network N" shows "start \<notin> interfaces N \<Longrightarrow> reachable N hdr start = {}"
-      apply(drule start_notininterfaces_succ_empty[OF wf_N])
-      apply(rule, rule)
-      apply(erule reachable_induct)
-      by(auto)
-    lemma succ_subseteq_reachable: "succ N start \<subseteq> reachable N hdr start"
-      by(auto intro: reachable.intros)
-
-
-    subsection{*The view of a packet*}
-      text{*For a fixed packet with a fixed header, its global network view is defined. 
-            For any start interface the packet is set out, the interfaces the packet can go next is recoreded.
-            
-            Essentially, view is a relation or the edges of a graph. This graph describes how the packet can move. 
-              The forwarding (and transfer) function is removed, the packet can directly move along the edges!
-
-            It is the view a packet has from the network.
-            *}
-      definition view :: "'v network \<Rightarrow> 'v hdr \<Rightarrow> (('v interface) \<times> ('v interface)) set" where
-        "view N hdr = {(src, dst). src \<in> interfaces N \<and> dst \<in> traverse N hdr src}"
-
-      text{*Alternative definition of view: For all interfaces in the network, collect the next hops. *}
-      lemma view_alt: "view N hdr = (\<Union>src \<in> interfaces N. {src} \<times> traverse N hdr src)"
-        apply(simp add: view_def)
-        apply(rule)
-        apply blast
-        apply(rule)
-        by(clarify)
-
-     lemma view_subseteq_interfaces_x_interfaces: assumes wf_N: "wellformed_network N"
-        shows "view N hdr \<subseteq> interfaces N \<times> interfaces N"
-        apply(simp add: view_alt)
-        using traverse_subseteq_interfaces[OF wf_N] by blast
-
-      lemma view_finite: assumes wf_N: "wellformed_network N"
-        shows "finite (view N hdr)"
-        apply(simp add: view_alt)
-        apply(subst finite_UN[OF wellformed_network.finite_interfaces[OF wf_N]])
-        apply(clarify)
-        apply(rule finite_cartesian_product)
-        apply simp
-        using traverse_finite[OF wf_N] by simp
-      lemma finite_view_trancl: assumes wf_N: "wellformed_network N" shows "finite ((view N hdr)\<^sup>+)"
-        using view_finite[OF wf_N] finite_trancl by simp
-
-      text{*The (bounded) reflexive transitive closure*}
-      (*In isabelle, saying only ^* would be transitive closure plus all reflexive elementes of type 'v interface. We only want all (interface N). 
-        For infinite types, ^* is infinite as it contains ALL {(a,a) | a of tpye}*)
-      definition view_rtrancl :: "'v network \<Rightarrow> 'v hdr \<Rightarrow> (('v interface) \<times> ('v interface)) set" where
-        "view_rtrancl N hdr \<equiv> {(src,dst). src \<in> interfaces N \<and> dst \<in> interfaces N \<and> (src, dst) \<in> (view N hdr)\<^sup>*}"
-
-      lemma assumes wf_N: "wellformed_network N" shows "finite (view_rtrancl N hdr)"
-        proof -
-          have "{(src,dst). src \<in> interfaces N \<and> dst \<in> interfaces N \<and> (src, dst) \<in> (view N hdr)\<^sup>*} \<subseteq> interfaces N \<times> interfaces N" by blast
-          thus ?thesis using wellformed_network.finite_interfaces[OF wf_N] unfolding view_rtrancl_def by (metis (lifting, no_types) finite_SigmaI rev_finite_subset)
-        qed
-
-      lemma view_rtrancl_alt: 
-        assumes wf_N: "wellformed_network N" shows "view_rtrancl N hdr = (view N hdr)\<^sup>+ \<union> {(a,a) | a . a \<in> interfaces N}"
-        unfolding view_rtrancl_def
-        apply(rule equalityI)
-        apply(clarify)
-        apply (metis rtranclD)
-        (* r to l*)
-        apply(clarify)
-        apply(rule)
-        apply(erule Set.UnE)
-        using view_subseteq_interfaces_x_interfaces[OF wf_N] apply (metis SigmaE2 converse_tranclE trancl_mono)
-        apply fastforce
-        apply(rule)
-        apply(erule Set.UnE)
-        using view_subseteq_interfaces_x_interfaces[OF wf_N] apply (metis mem_Sigma_iff r_into_trancl' subsetI subset_antisym trancl_mono trancl_subset_Sigma)
-        apply fastforce
-        apply(erule Set.UnE)
-        apply(simp)
-        apply(simp)
-        done
-    
-
-    lemma start_view_rtrancl:
-      assumes wf_N: "wellformed_network N"
-      shows "{dst. \<exists>first_hop \<in> succ N start. (first_hop, dst) \<in> (view N hdr)\<^sup>*} = (\<Union> first_hop \<in> succ N start. {dst. (first_hop, dst) \<in> (view N hdr)\<^sup>+}) \<union> (succ N start)" (is "?LHS = ?RHS")
-      proof -
-        have view_interfaces: "(view N hdr) `` (interfaces N) \<subseteq> (interfaces N)"
-          using view_subseteq_interfaces_x_interfaces[OF wf_N] by blast
-        have "?LHS \<subseteq> interfaces N"
-          apply(auto)
-          using succ_subseteq_interfaces[OF wf_N] Image_closed_trancl[OF view_interfaces] by auto
-        have "?LHS = {dst. \<exists>first_hop \<in> succ N start. (first_hop, dst) \<in> view_rtrancl N hdr}"
-          apply(simp add: view_rtrancl_def)
-          apply(rule Set.Collect_cong)
-          apply(rule iffI)
-          apply(erule bexE)
-          apply(rule_tac x="first_hop" in bexI)
-          apply(rule)
-          using succ_subseteq_interfaces[OF wf_N] apply blast
-          apply(rule)
-          using `?LHS \<subseteq> interfaces N` apply blast
-          apply(simp_all)
-          apply(erule bexE)
-          apply(rule_tac x="first_hop" in bexI)
-          by(simp_all)
-        also have "\<dots> = {dst. \<exists>first_hop \<in> succ N start. (first_hop, dst) \<in> (view N hdr)\<^sup>+} \<union> (succ N start)"
-          apply(subst view_rtrancl_alt[OF wf_N])
-          apply(rule)
-          apply fastforce
-          apply(rule)
-          apply(simp)
-          apply(erule disjE)
-          apply(erule bexE)
-          apply(rule_tac x="first_hop" in bexI)
-          apply(simp_all)
-          apply(rule_tac x="x" in bexI)
-          apply(simp_all)
-          using succ_subseteq_interfaces[OF wf_N] by blast
-        also have "\<dots> = (\<Union> first_hop \<in> succ N start. {dst. (first_hop, dst) \<in> (view N hdr)\<^sup>+}) \<union> (succ N start)"
-          by(simp add: Complete_Lattices.Collect_bex_eq)
-       finally show "?LHS = ?RHS" .
-     qed
-    (*lemma star_view_rtrancl:
-      assumes wf_N: "wellformed_network N"
-      and     start_iface: "start \<in> interfaces N"
-      shows "{dst. (start, dst) \<in> (view N hdr)\<^sup>*} = {dst. (start, dst) \<in> (view N hdr)\<^sup>+} \<union> {start}" (is "?LHS = ?RHS")
-      proof -
-        have "?LHS = {dst. (start, dst) \<in> view_rtrancl N hdr}"
-          unfolding view_rtrancl_def
-          apply(simp)
-          apply(auto simp add: start_iface)
-          using view_subseteq_interfaces_x_interfaces[OF wf_N] by (metis Image_closed_trancl Image_subset rev_ImageI start_iface)
-        also have "{dst. (start, dst) \<in> view_rtrancl N hdr} = ?RHS"
-         apply(subst view_rtrancl_alt[OF wf_N])
-         apply(rule)
-         apply fastforce
-         apply(rule)
-         apply(simp)
-         using start_iface apply fastforce
-         done
-       finally show "?LHS = ?RHS" .
-     qed*)
-     
-
-  section{*Reachable and view*}
-    text{*intuitive reachable definition and defining reachability by the rtrancl over the view relation is equal. *}
-    theorem reachable_eq_rtrancl_view:
-        assumes wf_N: "wellformed_network N"
-        shows "reachable N hdr start = {dst. \<exists>first_hop \<in> succ N start. (first_hop, dst) \<in> (view N hdr)\<^sup>*}"
-      proof(rule equalityI)
-        show "reachable N hdr start \<subseteq> {dst. \<exists>first_hop \<in> succ N start. (first_hop, dst) \<in> (view N hdr)\<^sup>*}"
-          proof(rule, simp)
-            fix x show "x \<in> reachable N hdr start \<Longrightarrow> \<exists>first_hop\<in>succ N start. (first_hop, x) \<in> (view N hdr)\<^sup>*"
-              proof(induction x rule:reachable_induct)
-                case(Start first_hop)
-                  hence "first_hop\<in>succ N start \<and> (first_hop, first_hop) \<in> (view N hdr)\<^sup>*" by(simp add: view_def)
-                  thus ?case by blast
-              next
-                case(Step hop next_hop)
-                  from reachable_subseteq_interfaces[OF wf_N] Step(1) have "hop \<in> interfaces N" by blast
-                  hence  "(hop, next_hop) \<in> {(src, dst). src \<in> interfaces N \<and> dst \<in> traverse N hdr src}"
-                    by(simp add: Step(2))
-                  hence  next_rtran: "(hop, next_hop) \<in> view N hdr"
-                    by(simp add: view_def)
-                  from Step(3) obtain first_hop where "first_hop\<in>succ N start" and first_rtran: "(first_hop, hop) \<in> (view N hdr)\<^sup>*" by blast
-                  from `first_hop\<in>succ N start` rtrancl.rtrancl_into_rtrancl[OF first_rtran next_rtran]
-                  show ?case by blast
-              qed
-         qed
-      next
-      show "{dst. \<exists>first_hop \<in> succ N start. (first_hop, dst) \<in> (view N hdr)\<^sup>*} \<subseteq> reachable N hdr start"   
-        proof(rule, clarify)
-          fix x first_hop
-          assume "first_hop \<in> succ N start"
-          show "(first_hop, x) \<in> (view N hdr)\<^sup>* \<Longrightarrow> x \<in> reachable N hdr start"
-            proof(induction rule: rtrancl_induct)
-              case base
-                thus ?case using reachable.intros(1) `first_hop \<in> succ N start` .
-              case(step y z)
-                thus ?case by(auto intro: reachable.intros(2) simp add: view_def)
-              qed
-            qed
-     qed
-    text{*reachability is exactly:
-      the first hop plus everything that can be transitively reached via the first hop. *}
-    corollary reachable_eq_rtrancl_view2:
-     "\<lbrakk> wellformed_network N \<rbrakk> \<Longrightarrow> reachable N hdr start = (\<Union> first_hop \<in> succ N start. {dst. (first_hop, dst) \<in> (view N hdr)\<^sup>+}) \<union> (succ N start)"
-     by(simp add: reachable_eq_rtrancl_view start_view_rtrancl)
+  (*traverse jumps over routers, it is not in the links. the forwarding function moves packets in routeres, there is no corresponding link IN an entity for it. *)
+  lemma traverse_subseteq_interfaces: "wellformed_network N \<Longrightarrow> traverse N hdr hop \<subseteq> interfaces N"
+    apply(simp add: traverse_def succ_def)
+    apply(drule wellformed_network.snd_links)
+    by force
+  corollary traverse_finite: assumes wf_N: "wellformed_network N"
+    shows "finite (traverse N hdr hop)"
+    using traverse_subseteq_interfaces[OF wf_N] wellformed_network.finite_interfaces[OF wf_N] by (metis rev_finite_subset)
 
 
 
-    lemma reachable_subset_start_iff:
-      assumes wf_N: "wellformed_network N"
-      shows only_reach_succ: "reachable N hdr start \<subseteq> succ N start \<longleftrightarrow> (\<forall>first_hop \<in> succ N start. traverse N hdr first_hop \<subseteq> succ N start)"
-      proof
-        assume only_reach_succ: "reachable N hdr start \<subseteq> succ N start"
-        show "\<forall>first_hop\<in>succ N start. traverse N hdr first_hop \<subseteq> succ N start"
-          proof 
-          fix first_hop
-          assume f: "first_hop \<in> succ N start"
-          from only_reach_succ have reach_eq_succ: "reachable N hdr start = succ N start" 
-            using Network.succ_subseteq_reachable by fast
-  
-          have view_dst_simp: "\<And> first_hop. {dst. first_hop \<in> interfaces N \<and> dst \<in> traverse N hdr first_hop} = 
-            {dst \<in> (\<Union>p\<in>forward N hdr first_hop. succ N \<lparr>entity = entity first_hop, port = p\<rparr>). first_hop \<in> interfaces N}"
-            by(simp only: traverse_def, blast)
-          
-          have "{dst. \<exists>first_hop \<in> succ N start. (first_hop, dst) \<in> (view N hdr)\<^sup>*} = 
-              (\<Union> first_hop \<in> succ N start. {dst. (first_hop, dst) \<in> (view N hdr)\<^sup>*})" by blast
-  
-          from this reach_eq_succ f have "{dst. (first_hop, dst) \<in> (view N hdr)\<^sup>*} \<subseteq> succ N start"
-            using reachable_eq_rtrancl_view[OF wf_N] by auto
-          
-          hence "{dst. (first_hop, dst) \<in> (view N hdr)} \<subseteq> succ N start" using f  by blast
-          hence "(\<Union>p\<in>forward N hdr first_hop. succ N \<lparr>entity = entity first_hop, port = p\<rparr>) \<subseteq> succ N start" using f
-            apply(simp add: view_def)                                          
-            apply(simp only: view_dst_simp)
-            by (metis reach_eq_succ reachable.simps subsetI traverse_def)
-          thus "traverse N hdr first_hop \<subseteq> succ N start"
-            by(simp add: traverse_def)
-          qed
-        next
-        assume only_traverse_succ: "\<forall>first_hop \<in> succ N start. traverse N hdr first_hop \<subseteq> succ N start"
-        {
-          fix x
-          have "x \<in> reachable N hdr start \<Longrightarrow> x \<in> succ N start"
-          proof(induction rule: reachable_induct)
-            case Start thus ?case by simp
-            next
-            case Step thus ?case using only_traverse_succ by fast
-          qed
-        }
-        thus "reachable N hdr start \<subseteq> succ N start" by blast
-      qed
+subsection {*Reachable interfaces*}
+  text{* Traverese performs one step to move a packet. The reachable set defines all reachable entities for a given start node of a packet. *}
+  (* we can allow spoofing by allowing an arbitrary packet header.*)
+  text{*reachable(1): a packet starts at a start node. All directly reachable nodes are reachable.
+        reachable(2): if a hop is reachables, then the next hop is also reachable. *}
+  inductive_set reachable :: "'v network \<Rightarrow> 'v hdr \<Rightarrow> 'v interface \<Rightarrow> ('v interface) set"
+  for N::"'v network" and "pkt_hdr"::"'v hdr" and "start"::"'v interface"
+  where
+    "first_hop \<in> succ N start \<Longrightarrow> first_hop \<in> reachable N pkt_hdr start" |
+    "hop \<in> reachable N pkt_hdr start \<Longrightarrow> next_hop \<in> (traverse N pkt_hdr hop) \<Longrightarrow> next_hop \<in> reachable N pkt_hdr start"
+
+  (*tuned induction rule*)
+  lemmas reachable_induct = reachable.induct[case_names Start Step]
+  thm reachable_induct
+
+  lemma reachable_subseteq_interfaces:
+    assumes wf_N: "wellformed_network N"
+    shows "reachable N pkt_hdr start \<subseteq> interfaces N"
+    proof
+      fix x
+      show "x \<in> reachable N pkt_hdr start \<Longrightarrow> x \<in> interfaces N"
+        apply(induction x rule: reachable_induct)
+        using succ_subseteq_interfaces[OF wf_N] apply blast
+        using traverse_subseteq_interfaces[OF wf_N] by fast
+    qed
+
+  lemma start_notininterfaces_reachableempty: assumes wf_N: "wellformed_network N" shows "start \<notin> interfaces N \<Longrightarrow> reachable N hdr start = {}"
+    apply(drule start_notininterfaces_succ_empty[OF wf_N])
+    apply(rule, rule)
+    apply(erule reachable_induct)
+    by(auto)
+  lemma succ_subseteq_reachable: "succ N start \<subseteq> reachable N hdr start"
+    by(auto intro: reachable.intros)
 
 
 
 
 
-  section{*Sending packets to hosts*}
-    text{*a packet from start is sent to dst. Which hosts gets the packet?*}
-    definition send_to :: "'v network \<Rightarrow> 'v interface \<Rightarrow> 'v entity \<Rightarrow> 'v interface set" where
-      "send_to N start dst \<equiv> hosts (reachable N (entity start, dst) start)"
+section{*Sending packets to hosts*}
+  text{*a packet from start is sent to dst. Which hosts gets the packet?*}
+  definition send_to :: "'v network \<Rightarrow> 'v interface \<Rightarrow> 'v entity \<Rightarrow> 'v interface set" where
+    "send_to N start dst \<equiv> hosts (reachable N (entity start, dst) start)"
 
 
-  section{*Can hosts spoof?*}
-    definition host_cannot_spoof :: "'v network \<Rightarrow> 'v interface \<Rightarrow> bool" where
-      "host_cannot_spoof N start \<equiv> \<forall> spoofed dst. spoofed \<noteq> entity start \<longrightarrow> reachable N (spoofed, dst) start \<subseteq> networkboxes (succ N start)"
 
-
-    (*if spoofed adresses exist ...*)
-    lemma "\<exists> spoofed. spoofed \<noteq> entity start \<Longrightarrow> host_cannot_spoof N start \<Longrightarrow> succ N start = networkboxes (succ N start)"
-      apply(rule succ_subset_networkboxes)
-      apply(simp add: host_cannot_spoof_def)
-      apply(erule exE)
-      using succ_subseteq_reachable by fast
-
-    (*if the adress space is so small that there is only one adress, a host cannot spoof (obviously)*)
-    lemma "\<not> (\<exists> spoofed. spoofed \<noteq> entity start) \<Longrightarrow> host_cannot_spoof N start"
-      by(simp add: host_cannot_spoof_def)
-      
-
-    text{*if all networkboxes connected to start block spoofing, start cannot spoof*}
-    lemma 
-      assumes connected_to_networkboxes: "succ N start = networkboxes (succ N start)" 
-        and   no_fwd_spoofed: "\<forall> spoofed dst. spoofed \<noteq> entity start \<longrightarrow> (\<forall> first_hop \<in> succ N start. (forward N (spoofed, dst) first_hop) = {})"
-      shows "host_cannot_spoof N start"
-      proof -
-        {
-        have "\<forall> spoofed dst. spoofed \<noteq> entity start \<longrightarrow> (\<forall> first_hop \<in> succ N start. (forward N (spoofed, dst) first_hop) = {}) \<Longrightarrow>
-                  host_cannot_spoof N start"
-        apply(simp add: host_cannot_spoof_def)
-        apply(clarify)
-        apply(erule reachable_induct)
-        apply(simp)
-        using connected_to_networkboxes apply fast
-        apply(simp add: traverse_def)
-        using connected_to_networkboxes apply blast
-        done
-        }
-        from this no_fwd_spoofed show ?thesis by simp
-      qed
-
-
-(*
-    lemma assumes wf_N: "wellformed_network N"
-      shows "host_cannot_spoof N start \<Longrightarrow> \<forall> spoofed dst. spoofed \<noteq> entity start \<longrightarrow> (\<forall> first_hop \<in> succ N start. (forward N (spoofed, dst) first_hop) = {})"
-      apply(simp add: host_cannot_spoof_def reachable_eq_rtrancl_view2[OF wf_N] view_def)
-      apply(clarsimp)
-      apply(erule allE)
-      apply(auto)
-      (*does not hold?  reachable start \<subseteq> succ start \<Longrightarrow> no forwarding to connected ports*)
-      oops
-*)
-  section{*Compliance with a Security Policy*}
+section{*Compliance with a Security Policy*}
     (*policy is a graph ... cannot spoof .... *)
 
 
-
-
-section{*TEST TEST TES TEST of UNIO*}
-  lemma "UNION {1::nat,2,3} (\<lambda>n. {n+1}) = {2,3,4}" by eval
-  lemma "(\<Union>n\<in>{1::nat, 2, 3}. {n + 1}) = {2, 3, 4}" by eval
-  lemma "UNION {1::nat,2,3} (\<lambda>n. {n+1}) = set (map (\<lambda>n. n+1) [1,2,3])" by eval
-
-(*
-  locale X =
-    fixes N1 N2
-    assumes well_n1: "wellformed_network N1"
-    assumes well_n2: "wellformed_network N2"
-  begin
-  end
-
-  sublocale X \<subseteq> n1!: wellformed_network N1
-    by (rule well_n1)
-  sublocale X \<subseteq> n2!: wellformed_network N2
-    by (rule well_n2)
-  
-    context X
-    begin
-      
-    end
-*)
 
 
 end
