interface_abstraction/Scratch.thy
@@ -1,0 +1,32 @@
+theory Scratch
+imports Main
+begin
+
+
+section{*TEST TEST TES TEST of UNIO*}
+  lemma "UNION {1::nat,2,3} (\<lambda>n. {n+1}) = {2,3,4}" by eval
+  lemma "(\<Union>n\<in>{1::nat, 2, 3}. {n + 1}) = {2, 3, 4}" by eval
+  lemma "UNION {1::nat,2,3} (\<lambda>n. {n+1}) = set (map (\<lambda>n. n+1) [1,2,3])" by eval
+
+(*
+  locale X =
+    fixes N1 N2
+    assumes well_n1: "wellformed_network N1"
+    assumes well_n2: "wellformed_network N2"
+  begin
+  end
+
+  sublocale X \<subseteq> n1!: wellformed_network N1
+    by (rule well_n1)
+  sublocale X \<subseteq> n2!: wellformed_network N2
+    by (rule well_n2)
+  
+    context X
+    begin
+      
+    end
+*)
+
+
+
+end
