interface_abstraction/Spoofing.thy
@@ -1,0 +1,56 @@
+theory Spoofing
+imports Network
+begin
+
+section{*Can hosts spoof?*}
+  definition host_cannot_spoof :: "'v network \<Rightarrow> 'v interface \<Rightarrow> bool" where
+    "host_cannot_spoof N start \<equiv> \<forall> spoofed dst. spoofed \<noteq> entity start \<longrightarrow> reachable N (spoofed, dst) start \<subseteq> networkboxes (succ N start)"
+
+
+  (*if spoofed adresses exist ...*)
+  lemma "\<exists> spoofed. spoofed \<noteq> entity start \<Longrightarrow> host_cannot_spoof N start \<Longrightarrow> succ N start = networkboxes (succ N start)"
+    apply(rule succ_subset_networkboxes)
+    apply(simp add: host_cannot_spoof_def)
+    apply(erule exE)
+    using succ_subseteq_reachable by fast
+
+  (*if the adress space is so small that there is only one adress, a host cannot spoof (obviously)*)
+  lemma "\<not> (\<exists> spoofed. spoofed \<noteq> entity start) \<Longrightarrow> host_cannot_spoof N start"
+    by(simp add: host_cannot_spoof_def)
+    
+
+  text{*if all networkboxes connected to start block spoofing, start cannot spoof*}
+  lemma 
+    assumes connected_to_networkboxes: "succ N start = networkboxes (succ N start)" 
+      and   no_fwd_spoofed: "\<forall> spoofed dst. spoofed \<noteq> entity start \<longrightarrow> (\<forall> first_hop \<in> succ N start. (forward N (spoofed, dst) first_hop) = {})"
+    shows "host_cannot_spoof N start"
+    proof -
+      {
+      have "\<forall> spoofed dst. spoofed \<noteq> entity start \<longrightarrow> (\<forall> first_hop \<in> succ N start. (forward N (spoofed, dst) first_hop) = {}) \<Longrightarrow>
+                host_cannot_spoof N start"
+      apply(simp add: host_cannot_spoof_def)
+      apply(clarify)
+      apply(erule reachable_induct)
+      apply(simp)
+      using connected_to_networkboxes apply fast
+      apply(simp add: traverse_def)
+      using connected_to_networkboxes apply blast
+      done
+      }
+      from this no_fwd_spoofed show ?thesis by simp
+    qed
+
+
+(*
+  lemma assumes wf_N: "wellformed_network N"
+    shows "host_cannot_spoof N start \<Longrightarrow> \<forall> spoofed dst. spoofed \<noteq> entity start \<longrightarrow> (\<forall> first_hop \<in> succ N start. (forward N (spoofed, dst) first_hop) = {})"
+    apply(simp add: host_cannot_spoof_def reachable_eq_rtrancl_view2[OF wf_N] view_def)
+    apply(clarsimp)
+    apply(erule allE)
+    apply(auto)
+    (*does not hold?  reachable start \<subseteq> succ start \<Longrightarrow> no forwarding to connected ports*)
+    oops
+*)
+
+
+end
